WIP; a small optimization to generate less declarations

code/curve25519/Hacl.Impl.Curve25519.Generic.fst
@@ -117,8 +117,7 @@ let encode_point #s o i =
   assert (as_seq h3 o == BSeq.nat_to_bytes_le 32 (feval h1 tmp));
   pop_frame()
 
-[@ Meta.Attribute.specialize ]
-assume val cswap2:
+val cswap2:
     #s:field_spec
   -> bit:uint64{v bit <= 1}
   -> p1:felem2 s
@@ -132,10 +131,10 @@ assume val cswap2:
       (v bit == 1 ==> as_seq h1 p1 == as_seq h0 p2 /\ as_seq h1 p2 == as_seq h0 p1) /\
       (v bit == 0 ==> as_seq h1 p1 == as_seq h0 p1 /\ as_seq h1 p2 == as_seq h0 p2) /\
       (fget_xz h1 p1, fget_xz h1 p2) == S.cswap2 bit (fget_xz h0 p1) (fget_xz h0 p2))
-(* let cswap2 #s bit p0 p1 =
+let cswap2 #s bit p0 p1 =
   match s with
   | M51 -> F51.cswap2 bit p0 p1
-  | M64 -> F64.cswap2 bit p0 p1 *)
+  | M64 -> F64.cswap2 bit p0 p1
 
 #set-options "--z3rlimit 150 --max_fuel 0 --max_ifuel 3"
 
@@ -171,7 +170,6 @@ val ladder_step:
       state_inv_t h1 (get_x q) /\ state_inv_t h1 (get_z q) /\
       state_inv_t h1 (get_x nq) /\ state_inv_t h1 (get_z nq) /\
       state_inv_t h1 (get_x nq_p1) /\ state_inv_t h1 (get_z nq_p1)))
-[@ Meta.Attribute.inline_ ]
 let ladder_step #s k q i p01_tmp1_swap tmp2 =
   let p01_tmp1 = sub p01_tmp1_swap 0ul (8ul *! nlimb s) in
   let swap : lbuffer uint64 1ul = sub p01_tmp1_swap (8ul *! nlimb s) 1ul in
@@ -227,7 +225,6 @@ val ladder_step_loop:
       v (LSeq.index (as_seq h1 bit) 0) <= 1 /\
       state_inv_t h1 (get_x nq) /\ state_inv_t h1 (get_z nq) /\
       state_inv_t h1 (get_x nq_p1) /\ state_inv_t h1 (get_z nq_p1)))
-[@ Meta.Attribute.inline_ ]
 let ladder_step_loop #s k q p01_tmp1_swap tmp2 =
   let h0 = ST.get () in
 
@@ -284,7 +281,6 @@ val ladder0_:
       state_inv_t h1 (get_x nq) /\ state_inv_t h1 (get_z nq) /\
       fget_xz h1 nq ==
       M.montgomery_ladder1_0 (as_seq h0 k) (fget_xz h0 q) (fget_xz h0 nq) (fget_xz h0 nq_p1)))
-[@ Meta.Attribute.inline_ ]
 let ladder0_ #s k q p01_tmp1_swap tmp2 =
   let p01_tmp1 = sub p01_tmp1_swap 0ul (8ul *! nlimb s) in
   let nq : point s = sub p01_tmp1_swap 0ul (2ul *! nlimb s) in
@@ -324,7 +320,6 @@ val ladder1_:
      (let nq = gsub p01_tmp1 0ul (2ul *! nlimb s) in
       state_inv_t h1 (get_x nq) /\ state_inv_t h1 (get_z nq) /\
       fget_xz h1 nq == M.montgomery_ladder1_1 (fget_xz h0 nq)))
-[@ Meta.Attribute.inline_ ]
 let ladder1_ #s p01_tmp1 tmp2 =
   let nq : point s = sub p01_tmp1 0ul (2ul *! nlimb s) in
   let tmp1 = sub p01_tmp1 (4ul *! nlimb s) (4ul *! nlimb s) in
@@ -359,7 +354,6 @@ val ladder2_:
       state_inv_t h1 (get_x nq) /\ state_inv_t h1 (get_z nq) /\
      (let nq' = M.montgomery_ladder1_0 (as_seq h0 k) (fget_xz h0 q) (fget_xz h0 nq) (fget_xz h0 nq_p1) in
       fget_xz h1 nq == M.montgomery_ladder1_1 nq')))
-[@ Meta.Attribute.inline_ ]
 let ladder2_ #s k q p01_tmp1_swap tmp2 =
   let p01_tmp1 = sub p01_tmp1_swap 0ul (8ul *! nlimb s) in
   let nq : point s = sub p01_tmp1_swap 0ul (2ul *! nlimb s) in
@@ -390,7 +384,6 @@ val ladder3_:
       state_inv_t h1 (get_x nq) /\ state_inv_t h1 (get_z nq) /\
       state_inv_t h1 (get_x nq_p1) /\ state_inv_t h1 (get_z nq_p1) /\
       (fget_xz h1 q, fget_xz h1 nq, fget_xz h1 nq_p1) == M.montgomery_ladder1_2 (fget_x h0 q)))
-[@ Meta.Attribute.inline_ ]
 let ladder3_ #s q p01 =
   let p0 : point s = sub p01 0ul (2ul *! nlimb s) in
   let p1 : point s = sub p01 (2ul *! nlimb s) (2ul *! nlimb s) in
@@ -432,7 +425,6 @@ val ladder4_:
      (let nq = gsub p01_tmp1_swap 0ul (2ul *! nlimb s) in
       state_inv_t h1 (get_x nq) /\ state_inv_t h1 (get_z nq) /\
       fget_xz h1 nq == S.montgomery_ladder (fget_x h0 q) (as_seq h0 k)))
-[@ Meta.Attribute.inline_ ]
 let ladder4_ #s k q p01_tmp1_swap tmp2 =
   let h0 = ST.get () in
   let p01 = sub p01_tmp1_swap 0ul (4ul *! nlimb s) in
