code/chacha20/Hacl.Chacha20.Vec128.fst
@@ -3,11 +3,11 @@ module Hacl.Chacha20.Vec128
 open Hacl.Meta.Chacha20.Vec
 
 private
-let double_round_128 = double_round_higher #4
+let double_round_128 = Hacl.Impl.Chacha20.Core32xN.double_round #4
 private
 let chacha20_core_128 = chacha20_core_higher #4 double_round_128
 private
-let chacha20_init_128 = chacha20_init_higher #4
+let chacha20_init_128 = Hacl.Impl.Chacha20.Vec.chacha20_init #4
 
 let chacha20_encrypt_128 = chacha20_encrypt_higher #4 chacha20_init_128 chacha20_core_128
 let chacha20_decrypt_128 = chacha20_decrypt_higher #4 chacha20_init_128 chacha20_core_128
