code/chacha20poly1305/Hacl.Meta.Chacha20Poly1305.fst
@@ -3,7 +3,6 @@ module Hacl.Meta.Chacha20Poly1305
 #set-options "--z3rlimit 250 --max_fuel 0 --max_ifuel 1"
 
 %splice[
-  poly1305_padded_higher;
   poly1305_do_higher;
   aead_encrypt_higher;
   aead_decrypt_higher
